Main.v
@@ -12,41 +12,6 @@
 
 (* abbreviations and ideas:
   CBT        crit-bit tree (we usually mean this to be a *non-empty* crit-bit tree)
-
-  augCBT     augmented crit-bit tree:
-             For the purposes of the proofs, we augment the basic CBT with additional data.
-             Specifically, we store the full current prefix at every internal node.
-             There is a natural bijection between valid CBTs and valid augCBTs. (Given a CBT,
-             we can construct the *unique* augmenting data. Given a augCBT, we can just forget
-             the augmenting data. This latter direction of the bijection is obviously much easier
-             to compute -- we call it stripping -- see strip_augCBT.)
-             A CBT is defined to be valid iff it can be obtained by stripping some valid augCBT.
-             The core property of a valid augCBT is that for an internal node with prefix p,
-             p ++ [false] is a prefix of the left child's prefix and p ++ [true] is a prefix of the
-             right child's prefix.
-
-             In general, this permits the following high-level structure of proofs about properties of
-             operations on CBTs.
-             - For an operation defined as op: CBT -> CBT, define this operation in a more convenient way
-               as aug_op: augCBT -> augCBT.
-             - Prove that these two 'do the same thing':
-
-                   aut  -- aug_op -->   aut'
-
-                    |                    |
-                  strip                strip
-                    |                    |
-                    v                    v
-
-                    t   --  op    -->    t'
-
-
-                    commutes (if aut is valid)
-
-             - Prove that aug_op has the desired functional properties.
-
-  content    We define the keys and values that a CBT / augCBT contains in terms of
-             what the lookup function returns.
 *)
 
 Require Import List.
@@ -54,6 +19,7 @@ Require Import Nat.
 Require Import Bool.
 Require Import Arith.
 Require Import Arith.Compare.
+Require Import Logic.FunctionalExtensionality.
 Import ListNotations.
 
 From CritBit Require Import Front.
@@ -62,447 +28,374 @@ From CritBit Require Import KeyUtil.
 From CritBit Require Import PrefixCritical.
 From CritBit Require Import SeqAccess.
 
-(* an augmented CBT tree (non-empty) *)
-Inductive augCBT {X : Type} : Type :=
-  | AugLeaf (k : list bool) (v : X)
-  | AugBranch (p : list bool) (l r : augCBT).
+Definition content_map (X : Type) : Type := list bool -> option X.
 
-(* strip an augCBT -- forget the augmenting data *)
-Fixpoint strip_augCBT {X : Type} (t : @augCBT X) : CBT :=
-  match t with
-  | AugLeaf k v => Leaf k v
-  | AugBranch p l r => Branch (length p) (strip_augCBT l) (strip_augCBT r)
-  end.
+Definition singleton {X : Type} (k : list bool) (v : X) : content_map X
+  := fun k' => if key_eqb k k' then Some v else None.
 
-Definition prefix_from_aug {X : Type} (aut : @augCBT X) : prefix :=
-  match aut with
-  | AugLeaf k _ => ZeroExt k
-  | AugBranch k _ _ => Finite k
-  end.
+Definition cbit_union {X : Type} (cbit : nat) (m0 m1 : content_map X) : content_map X
+  := fun k' => if ith_zer cbit k' then m1 k' else m0 k'.
 
-Inductive augCBT_valid {X : Type} : augCBT -> Prop :=
-  | acv_leaf (k : list bool) (v : X) (H: OneTerminated k)
-      : augCBT_valid (AugLeaf k v)
-  | acv_branch (p : list bool) (l r : augCBT)
-    (H1: augCBT_valid l) (H2: is_prefix (p ++ (false :: nil)) (prefix_from_aug l))
-    (H3: augCBT_valid r) (H4: is_prefix (p ++ (true :: nil)) (prefix_from_aug r))
-      : augCBT_valid (AugBranch p l r).
+Inductive pmCBT_valid {X : Type} : prefix -> content_map X -> @CBT X -> Prop :=
+| pcv_leaf (k : list bool) (v : X) (H : OneTerminated k)
+  : pmCBT_valid (ZeroExt k) (singleton k v) (Leaf k v)
+| pcv_branch (p : list bool) (pl pr : prefix) (ml mr : content_map X) (l r : CBT)
+    (Hl : pmCBT_valid pl ml l) (Hr : pmCBT_valid pr mr r)
+    (Hpl : is_prefix (p ++ [false]) pl) (Hpr : is_prefix (p ++ [true]) pr)
+  : pmCBT_valid (Finite p) (cbit_union (length p) ml mr) (Branch (length p) l r).
 
-Inductive CBT_valid {X : Type} : (@CBT X) -> Prop :=
-  | cv (t : CBT) (aut : augCBT)
-    (H1: strip_augCBT aut = t) (H2: augCBT_valid aut) : CBT_valid t.
+Definition pCBT_valid {X : Type} (p : prefix) (t : @CBT X) : Prop :=
+  exists m, pmCBT_valid p m t.
 
-Definition content_aug {X : Type} (aut : augCBT) (k : list bool) := @lookup X k (strip_augCBT aut).
-
-Lemma find_key_has_prefix : forall (X : Type) (k p : list bool) (l r : augCBT),
-  (augCBT_valid (AugBranch p l r)) ->
-  (is_prefix_zer p (@find_best_key X k (strip_augCBT (AugBranch p l r)))).
+Lemma pmCBT_valid_forget_m : forall (X : Type)
+                                    (p : prefix) (m : content_map X) (t : CBT),
+    pmCBT_valid p m t -> pCBT_valid p t.
 Proof.
-  intros X k p l r E.
-  remember (AugBranch p l r) as aut.
-  generalize dependent p. generalize dependent l. generalize dependent r.
-  induction E.
-  - intros r l p H2. discriminate.
-  - intros r' l' p' H3. injection H3 as H3. rewrite <- H3 in *.
-    clear H3 H H0 p' l' r'. simpl. destruct (ith_zer (length p) k).
-    + clear IHE1 E1 H2 l. inversion E2.
-      * simpl. rewrite <- H0 in H4. simpl in H4. apply app_is_prefix_zer in H4.
-        exact H4.
-      * symmetry in H. specialize (IHE2 r0 l p0 H). rewrite H in H4. simpl in H4.
-        apply app_is_prefix_fin in H4. apply prefix_zer_trans with p0. exact H4.
-        rewrite H in IHE2. exact IHE2.
-    + clear IHE2 E2 H4 r. inversion E1.
-      * simpl. rewrite <- H0 in H2. simpl in H2. apply app_is_prefix_zer in H2.
-        exact H2.
-      * symmetry in H. specialize (IHE1 r l0 p0 H). rewrite H in H2. simpl in H2.
-        apply app_is_prefix_fin in H2. apply prefix_zer_trans with p0. exact H2.
-        rewrite H in IHE1. exact IHE1.
+  intros X p m t H. exists m. assumption.
 Qed.
 
-Fixpoint critical_bit_augCBT {X : Type} (k : list bool) (aut : @augCBT X) : option nat :=
-  match aut with
-  | AugLeaf k' _ => critical_bit_zer k' k
-  | AugBranch p l r => if is_prefix_zerb p k then
-      if ith_zer (length p) k then
-        critical_bit_augCBT k r
+Definition mCBT_valid {X : Type} (m : content_map X) (t : @CBT X) : Prop :=
+  exists p, pmCBT_valid p m t.
+
+Lemma pmCBT_valid_forget_p : forall (X : Type)
+                                    (p : prefix) (m : content_map X) (t : CBT),
+    pmCBT_valid p m t -> mCBT_valid m t.
+Proof.
+  intros. exists p. assumption.
+Qed.
+
+Definition CBT_valid {X : Type} (t : @CBT X) : Prop :=
+  exists p m, pmCBT_valid p m t.
+
+(* ROOM FOR IMPROVEMENT: prove this lemma using the one one below and
+   a lemma that the best key is in the content map *)
+Lemma best_key_has_prefix : forall (X : Type) (k p : list bool)
+                                   (t : @CBT X),
+    pCBT_valid (Finite p) t ->
+    is_prefix_zer p (find_best_key k t).
+Proof.
+  intros X k p t. generalize dependent p. induction t.
+  - intros p H. destruct H. inversion H.
+  - intros p H. simpl. destruct H as [m H]. inversion H. rewrite <- H3 in H.
+    clear l r H3 H4 H5 p0 H1 i H0.
+    destruct (ith_zer (length p) k) eqn:E.
+    + clear IHt1 t1 Hpl pl Hl H. destruct pr eqn:E2.
+      * inversion Hr. simpl in *. apply app_is_prefix_zer in Hpr. assumption.
+      * apply pmCBT_valid_forget_m in Hr. specialize (IHt2 p0 Hr).
+        apply app_is_prefix in Hpr. simpl in Hpr.
+        apply (prefix_zer_trans p p0 _ Hpr IHt2).
+    + clear IHt2 t2 Hpr pr Hr H. destruct pl eqn:E2.
+      * inversion Hl. simpl in *. apply app_is_prefix_zer in Hpl. assumption.
+      * apply pmCBT_valid_forget_m in Hl. specialize (IHt1 p0 Hl).
+        apply app_is_prefix in Hpl. simpl in Hpl.
+        apply (prefix_zer_trans p p0 _ Hpl IHt1).
+Qed.
+
+Lemma key_has_prefix : forall (X : Type) (k p : list bool) (m : content_map X)
+                                (t : CBT),
+    pmCBT_valid (Finite p) m t -> (exists v, m k = Some v) -> is_prefix_zer p k.
+Proof.
+  intros. remember (Finite p) as pi. generalize dependent p.
+  induction H; intros p1 H2.
+  - discriminate.
+  - destruct H0 as [v H0]. unfold cbit_union in H0. injection H2 as H2. subst p1.
+    destruct (ith_zer (length p) k).
+    + clear IHpmCBT_valid1 Hpl H l. apply app_is_prefix in Hpr.
+      destruct pr eqn:E; simpl in Hpr.
+      * inversion H1. subst. unfold singleton in H0. destruct (key_eqb p0 k) eqn:E.
+        apply key_eqb_iff in E. subst p0. assumption. discriminate.
+      * assert (exists v : X, mr k = Some v). exists v. assumption.
+        specialize (IHpmCBT_valid2 H p0 (eq_refl (Finite p0))).
+        eapply prefix_zer_trans. eassumption. assumption.
+    + clear IHpmCBT_valid2 Hpr H1 r. apply app_is_prefix in Hpl.
+      destruct pl eqn:E; simpl in Hpl.
+      * inversion H. subst. unfold singleton in H0. destruct (key_eqb p0 k) eqn:E;
+          try discriminate. apply key_eqb_iff in E. subst p0. assumption.
+      * assert (exists v, ml k = Some v). exists v. assumption.
+        specialize (IHpmCBT_valid1 H1 p0 (eq_refl (Finite p0))).
+        eapply prefix_zer_trans. eassumption. assumption.
+Qed.
+
+Lemma best_key_one_terminated : forall (X : Type) (k : list bool) (t : @CBT X),
+    CBT_valid t -> OneTerminated (find_best_key k t).
+Proof.
+  induction t.
+  - intro H. unfold CBT_valid in H. destruct H as [m [p H]]. inversion H. simpl.
+    assumption.
+  - intro H. simpl. unfold CBT_valid in *. destruct H as [m [p0 H]]. inversion H. rewrite <- H3 in *.
+    destruct (ith_zer (length p) k).
+    + apply IHt2. exists pr. exists mr. assumption.
+    + apply IHt1. exists pl. exists ml. assumption.
+Qed.
+
+Lemma is_beforeb_true_exists : forall (o : option nat) (m : nat),
+    is_beforeb o m = true -> exists n, o = Some n /\ S n <= m.
+Proof.
+  intros o m H. destruct o.
+  - simpl in H. exists n. split. reflexivity. apply Nat.ltb_lt in H.
+    unfold "<" in H. assumption.
+  - discriminate.
+Qed.
+
+Lemma is_beforeb_false_high_none : forall (o : option nat) (m : nat),
+    is_beforeb o m = false -> (o = None \/ exists n, o = Some n /\ m <= n).
+Proof.
+  intros o m H. destruct o.
+  - simpl in H. right. exists n. split. reflexivity. apply Nat.ltb_ge. assumption.
+  - left. reflexivity.
+Qed.
+
+Lemma high_critbit_is_prefix : forall (X : Type) (k p : list bool) (t : @CBT X),
+    pCBT_valid (Finite p) t ->
+    is_beforeb (critical_bit_CBT k t) (length p) = false ->
+    is_prefix_zer p k.
+Proof.
+  intros X k p t H1 H2. destruct H1 as [m H1]. inversion H1. rewrite <- H4 in *.
+  clear t H4 p0 H0 H3. apply is_beforeb_false_high_none in H2.
+  apply pmCBT_valid_forget_m in H1. apply best_key_has_prefix with (k:=k) in H1.
+  apply prefix_iff_take_eq in H1. unfold critical_bit_CBT in H2.
+  remember (find_best_key k (Branch (length p) l r)) as k'.
+  assert (take_zer (length p) k = take_zer (length p) k').
+  { destruct H2.
+    - rewrite critical_bit_zer_none_eqv in H. specialize (H (length p)). assumption.
+    - destruct H as [n [H2 H3]]. apply critical_bit_zer_take_eq in H2.
+      rewrite <- (take_take _ n _). rewrite H2. rewrite take_take. reflexivity.
+      assumption. assumption. }
+  apply prefix_iff_take_eq. rewrite H. assumption.
+Qed.
+
+Lemma low_critbit_on_prefix : forall (X : Type) (k p : list bool) (t : @CBT X),
+    pCBT_valid (Finite p) t ->
+    is_beforeb (critical_bit_CBT k t) (length p) = true ->
+    critical_bit_CBT k t = critical_bit_fin k p.
+Proof.
+  intros X k p t. generalize dependent p. induction t.
+  - intros p H. destruct H. inversion H.
+  - intros p H1 H2. unfold critical_bit_CBT in *. simpl in *. destruct H1 as [m H1].
+    inversion H1. rewrite <- H in *. clear H5 l H6 r H0 p0 H i.
+    apply app_is_prefix in Hpl. apply app_is_prefix in Hpr.
+    assert (forall (ps : prefix) (t : @CBT X),
+               (forall (p : list bool), pCBT_valid (Finite p) t ->
+                                      is_beforeb (critical_bit_zer k (find_best_key k t)) (length p) = true ->
+                                      critical_bit_zer k (find_best_key k t) = critical_bit_fin k p) ->
+               is_beforeb (critical_bit_zer k (find_best_key k t)) (length p) = true ->
+               is_prefix p ps ->
+               pCBT_valid ps t ->
+               critical_bit_zer k (find_best_key k t) = critical_bit_fin k p). {
+      clear. intros ps t H1 H2 H3 H4. apply is_beforeb_true_exists in H2.
+      destruct H2 as [n [H5 H6]]. destruct ps.
+      - destruct H4 as [m H4]. inversion H4. rewrite <- H7 in *. clear H k0 H4 H7 t H2.
+        simpl in *. rewrite H5.
+        symmetry. apply critical_bit_zer_fin. assumption.
+        apply prefix_iff_take_eq in H3. rewrite <- H3. apply critical_bit_zer_from_parts.
+        apply critical_bit_zer_take_eq in H5. rewrite take_take.
+        assumption. apply Le.le_Sn_le_stt. assumption. rewrite ith_from_take.
+        apply critical_bit_zer_ith_neq in H5. assumption. assumption.
+      - specialize (H1 p0 H4).
+        pose proof (best_key_has_prefix X k p0 t H4).
+        remember (find_best_key k t) as k'. clear Heqk' H4. simpl in H3.
+        rewrite H5 in *. clear H5. simpl in H1. rewrite Nat.ltb_lt in H1.
+        unfold "<" in H1. assert (S n <= length p0). transitivity (length p).
+        assumption. apply is_prefix_fin_length. assumption. specialize (H1 H0).
+        symmetry. symmetry in H1. apply critical_bit_fin_zer in H1.
+        apply critical_bit_zer_fin. assumption. apply is_prefix_fin_zer in H3.
+        apply prefix_iff_take_eq in H3. rewrite <- H3.
+        apply critical_bit_zer_from_parts. rewrite take_take.
+        apply critical_bit_zer_take_eq in H1. assumption. apply Le.le_Sn_le_stt.
+        assumption. rewrite ith_from_take. apply critical_bit_zer_ith_neq in H1.
+        assumption. assumption.
+    } destruct (ith_zer (length p) k).
+    + apply pmCBT_valid_forget_m in Hr. apply (H pr t2 IHt2 H2 Hpr Hr).
+    + apply pmCBT_valid_forget_m in Hl. apply (H pl t1 IHt1 H2 Hpl Hl).
+Qed.
+
+Lemma pcv_finite_len_num : forall (X : Type) (p : list bool) (plen : nat)
+                                  (pl pr : prefix) (l r : CBT),
+    length p = plen -> is_prefix (p ++ [false]) pl -> is_prefix (p ++ [true]) pr ->
+    pCBT_valid pl l -> pCBT_valid pr r -> @pCBT_valid X (Finite p) (Branch plen l r).
+Proof.
+  intros *. intros H1 H2 H3 H4 H5. rewrite <- H1.
+  destruct H4 as [ml H4]. destruct H5 as [mr H5].
+  exists (fun k' => if ith_zer (length p) k' then mr k' else ml k').
+  apply pcv_branch with (pl:=pl) (pr:=pr).
+  assumption. assumption. assumption. assumption.
+Qed.
+
+Lemma pmcv_finite_len_num : forall (X : Type) (p : list bool) (plen : nat)
+                                   (pl pr : prefix) (ml mr : content_map X) (l r : CBT),
+    length p = plen -> is_prefix (p ++ [false]) pl -> is_prefix (p ++ [true]) pr ->
+    pmCBT_valid pl ml l -> pmCBT_valid pr mr r ->
+    pmCBT_valid (Finite p) (cbit_union plen ml mr) (Branch plen l r).
+Proof.
+  intros. rewrite <- H. econstructor; eassumption.
+Qed.
+
+Definition cmap_insert {X : Type} (k : list bool) (v : X) (m : content_map X)
+  : content_map X := (fun k' => if key_eqb k k' then Some v else m k').
+
+Lemma cmap_insert_cbit_singleton : forall (X : Type) (k0 k : list bool) (v0 v : X)
+                                          (n : nat),
+    critical_bit_zer k k0 = Some n ->
+    cmap_insert k v (singleton k0 v0) = if ith_zer n k then
+                                          cbit_union n (singleton k0 v0) (singleton k v)
+                                        else
+                                          cbit_union n (singleton k v) (singleton k0 v0).
+Proof.
+  intros X k0 k v0 v n H1. unfold cmap_insert. unfold cbit_union.
+  apply critical_bit_zer_ith_neq in H1. extensionality k''. unfold singleton.
+  destruct (key_eqb k k'') eqn:E.
+  - apply key_eqb_iff in E. subst k''.
+    destruct (ith_zer n k) eqn:E2; apply not_eq_sym in H1; rewrite E2;
+    rewrite (key_eqb_reflx k); reflexivity.
+  - destruct (ith_zer n k) eqn:E2; apply bneq_eq_neg in H1; symmetry in H1; simpl in H1;
+    rewrite E; destruct (key_eqb k0 k'') eqn:E3; try (apply key_eqb_iff in E3; subst;
+    rewrite H1; reflexivity); destruct (ith_zer n k''); reflexivity.
+Qed.
+
+Lemma cmap_insert_eqk_singleton : forall (X : Type) (k : list bool) (v0 v : X),
+  cmap_insert k v (singleton k v0) = singleton k v.
+Proof.
+  intros. extensionality k'. unfold cmap_insert. unfold singleton.
+  destruct (key_eqb k k'); reflexivity.
+Qed.
+
+Lemma cmap_insert_low_cb_branch : forall (X : Type) (k : list bool) (v : X)
+                                         (p : list bool) (m : content_map X)
+                                         (l r : @CBT X) (n : nat),
+    pmCBT_valid (Finite p) m (Branch (length p) l r) ->
+    critical_bit_CBT k (Branch (length p) l r) = Some n -> n < length p ->
+    cmap_insert k v m = if ith_zer n k then
+                          cbit_union n m (singleton k v)
+                        else
+                          cbit_union n (singleton k v) m.
+Proof.
+  intros. unfold cmap_insert. extensionality k0. unfold cbit_union.
+  destruct (key_eqb k k0) eqn:E.
+  - apply key_eqb_iff in E. subst k0. destruct (ith_zer n k) eqn:E;
+      rewrite E; unfold singleton; rewrite key_eqb_reflx; reflexivity.
+  - destruct (m k0) eqn:E2.
+    + assert (exists v, m k0 = Some v). exists x. assumption.
+      eapply key_has_prefix in H2; try eassumption.
+      assert (ith_zer n k <> ith_zer n p).
+      { apply pmCBT_valid_forget_m in H. eapply low_critbit_on_prefix in H.
+        rewrite H0 in H. symmetry in H. apply critical_bit_fin_zer in H.
+        apply critical_bit_zer_ith_neq in H. assumption.
+        rewrite H0. simpl. apply Nat.ltb_lt. assumption. }
+      destruct (ith_zer n k); apply bneq_eq_neg in H3; destruct (ith_zer n k0) eqn:E4;
+        try (symmetry; assumption); unfold singleton; rewrite E;
+        apply prefix_iff_take_eq in H2; eapply ith_from_take in H1; rewrite H2 in H1;
+        rewrite E4 in H1; rewrite <- H3 in H1; discriminate.
+    + unfold singleton. destruct (ith_zer n k); rewrite E2; rewrite E;
+        destruct (ith_zer n k0); reflexivity.
+Qed.
+
+Lemma cmap_insert_high_cb_branch : forall (X : Type) (k : list bool) (v : X)
+                                          (p : list bool) (ml mr : content_map X)
+                                          (l r : @CBT X),
+    pmCBT_valid (Finite p) (cbit_union (length p) ml mr) (Branch (length p) l r) ->
+    is_beforeb (critical_bit_CBT k (Branch (length p) l r)) (length p) = false ->
+    cmap_insert k v (cbit_union (length p) ml mr)
+    = if ith_zer (length p) k then
+        cbit_union (length p) ml (cmap_insert k v mr)
       else
-        critical_bit_augCBT k l
-    else
-      critical_bit_zer p k
-  end.
-
-Lemma critical_bit_aug_match : forall (X : Type) (k : list bool) (aut : @augCBT X),
-  (augCBT_valid aut) -> (critical_bit_augCBT k aut = critical_bit_CBT k (strip_augCBT aut)).
+        cbit_union (length p) (cmap_insert k v ml) mr.
 Proof.
-  induction aut as [k' v | p' l IHl r IHr ].
-  - intro H. unfold critical_bit_CBT. simpl. apply critical_bit_zer_comm.
-  - unfold critical_bit_CBT in IHl. unfold critical_bit_CBT in IHr. unfold critical_bit_CBT.
-    intro H. simpl. destruct (is_prefix_zerb p' k) eqn:E.
-    + inversion H. destruct (ith_zer (length p') k) eqn:E2.
-      * apply IHr. exact H5.
-      * apply IHl. exact H0.
-    + remember (find_best_key k (if ith_zer (length p') k then strip_augCBT r else strip_augCBT l)) as fb.
-      assert (fb = find_best_key k (strip_augCBT (AugBranch p' l r))). { simpl. exact Heqfb. }
-      assert (is_prefix_zer p' fb). { rewrite H0. apply find_key_has_prefix. exact H. }
-      symmetry. destruct (critical_bit_zer p' k) eqn:E2.
-      * assert (S n <= length p').
-        { assert ({S n <= length p'} + {length p' <= S n}). apply le_dec. destruct H2. exact l0.
-        apply le_decide in l0. unfold lt_or_eq in l0. destruct l0. unfold ">" in g. unfold "<" in g.
-        apply le_S_n in g. apply critical_bit_zer_take_eq in E2.
-        assert (take_zer (length p') p' = take_zer (length p') k). rewrite <- (take_take (length p') n p').
-        rewrite <- (take_take (length p') n k). rewrite E2. reflexivity. exact g. exact g.
-        rewrite take_full in H2. symmetry in H2. apply prefix_iff_take_eq in H2.
-        apply is_prefix_zer_iff in H2. rewrite H2 in E. discriminate. rewrite e. apply le_n. }
-        assert (n <= length p'). { apply le_S in H2. apply le_S_n in H2. exact H2. }
-        apply critical_bit_zer_from_parts.
-       -- apply critical_bit_zer_take_eq in E2. apply prefix_iff_take_eq in H1.
-          assert (take_zer n fb = take_zer n p'). { rewrite <- (take_take n (length p') fb).
-          rewrite H1. reflexivity. exact H3. } symmetry. transitivity (take_zer n p').
-          exact H4. exact E2.
-       -- apply critical_bit_zer_ith_neq in E2. assert (ith_zer n p' = ith_zer n fb).
-          { rewrite <- (ith_from_take n (length p') fb). apply prefix_iff_take_eq in H1.
-          rewrite H1. reflexivity. exact H2. } intro H5. apply E2. symmetry in H5.
-          transitivity (ith_zer n fb). exact H4. exact H5.
-      * apply critical_bit_zer_none_prefix in E2. apply is_prefix_zer_iff in E2.
-        rewrite E2 in E. discriminate.
+  intros.
+  apply high_critbit_is_prefix in H0; try (eapply pmCBT_valid_forget_m; eassumption).
+  unfold cmap_insert. unfold cbit_union. extensionality k0.
+  destruct (ith_zer (length p) k) eqn:E2; destruct (key_eqb k k0) eqn:E;
+    try (apply key_eqb_iff in E; subst k0); try rewrite E2; try reflexivity.
 Qed.
 
-Lemma critical_bit_augCBT_increasing : forall (X : Type) (k p : list bool) (l r : augCBT),
-  (augCBT_valid (AugBranch p l r)) ->
-  (is_prefix_zer p k) ->
-  (is_beforeb (@critical_bit_augCBT X k (AugBranch p l r)) (length p) = false).
+Theorem insert_correct {X : Type} :
+  forall (p : prefix) (m : content_map X) (t : CBT) (k : list bool) (v : X)
+         (p' : list bool),
+    pmCBT_valid p m t -> is_prefix p' p -> is_prefix_zer p' k -> OneTerminated k ->
+    exists pi, is_prefix p' pi /\ pmCBT_valid pi (cmap_insert k v m) (insert k v t).
 Proof.
-  intros X k p l r E. remember (AugBranch p l r) as aut.
-  generalize dependent p. generalize dependent l. generalize dependent r.
-  induction E.
-  - intros r l p H2 H3. discriminate.
-  - intros r' l' p' H3 H5. injection H3 as H3. rewrite <- H3 in *. clear H3 H H0 p' l' r'.
-    unfold is_beforeb. simpl. apply is_prefix_zer_iff in H5. rewrite H5.
-    assert (HS: forall (aut : augCBT),
-      (augCBT_valid aut) -> (is_prefix p (prefix_from_aug aut)) ->
-      (forall (r' l' : augCBT) (p' : list bool),
-        aut = AugBranch p' l' r' -> is_prefix_zer p' k -> is_beforeb (@critical_bit_augCBT X k aut) (length p') = false)
-      -> match critical_bit_augCBT k aut with
-         | Some i => i <? length p
-         | None => false
-        end = false). {
-      clear IHE1 IHE2 E1 H2 E2 H4 l r. intros aut H1 H2 IH. destruct aut.
-      - simpl. simpl in H2. destruct (critical_bit_zer k0 k) eqn:E3.
-        apply Nat.ltb_ge. apply is_prefix_zer_iff in H5. apply (same_prefix_zer p k0 k) in H2.
-        apply (critical_bit_zer_after k0 k). exact H2. exact E3. exact H5. reflexivity.
-      - simpl. simpl in H2. destruct (is_prefix_zerb p0 k) eqn:E3.
-       -- assert (AugBranch p0 aut1 aut2 = AugBranch p0 aut1 aut2). reflexivity.
-          apply is_prefix_fin_length in H2. apply is_prefix_zer_iff in E3.
-          specialize (IH aut2 aut1 p0 H E3). unfold is_beforeb in IH. simpl in IH.
-          apply is_prefix_zer_iff in E3. rewrite E3 in IH. destruct (ith_zer (length p0) k) eqn:E4.
-         ++ destruct (critical_bit_augCBT k aut2) eqn:E5.
-            apply Nat.ltb_ge. apply Nat.ltb_ge in IH. apply Nat.le_trans with (length p0).
-            exact H2. exact IH. reflexivity.
-         ++ destruct (critical_bit_augCBT k aut1) eqn:E5.
-            apply Nat.ltb_ge. apply Nat.ltb_ge in IH. apply Nat.le_trans with (length p0).
-            exact H2. exact IH. reflexivity.
-       -- destruct (critical_bit_zer p0 k) eqn:E4. apply Nat.ltb_ge. apply is_prefix_zer_iff in H5.
-          apply prefix_iff_take_eq in H5. apply (critical_bit_zer_after p0 k).
-          apply is_prefix_fin_zer in H2. apply prefix_iff_take_eq in H2.
-          rewrite H2. symmetry. exact H5. exact E4. reflexivity.
-    }
-    destruct (ith_zer (length p) k).
-    + apply (HS r E2 (app_is_prefix p [true] _ H4) IHE2).
-    + apply (HS l E1 (app_is_prefix p [false] _ H2) IHE1).
-Qed.
- 
-Definition insert_as_branch_aug {X : Type} (k : list bool) (v : X) (i : nat) (aut : augCBT) : augCBT :=
-  if ith_zer i k then AugBranch (take_zer i k) aut (AugLeaf k v) else AugBranch (take_zer i k) (AugLeaf k v) aut.
-
-Fixpoint insert_aug {X : Type} (k : list bool) (v : X) (aut : augCBT) : augCBT :=
-  match aut with
-  | AugLeaf k' _ =>
-    match critical_bit_zer k' k with
-    | None => AugLeaf k' v
-    | Some cbit => insert_as_branch_aug k v cbit aut
-    end
-  | AugBranch p l r =>
-    match critical_bit_fin k p with
-    | None => if ith_zer (length p) k
-      then AugBranch p l (insert_aug k v r)
-      else AugBranch p (insert_aug k v l) r
-    | Some cbit => insert_as_branch_aug k v cbit aut
-    end
-  end.
-
-Lemma insert_aug_match : forall (X : Type) (k : list bool) (v : X) (aut : augCBT) (p : list bool),
-  (OneTerminated k) ->
-  (augCBT_valid aut) ->
-  (is_prefix_zer p k) ->
-  (is_prefix p (prefix_from_aug aut)) ->
-  (
-    augCBT_valid (insert_aug k v aut)
-    /\ strip_augCBT (insert_aug k v aut) = insert_at k v (critical_bit_augCBT k aut) (strip_augCBT aut)
-    /\ is_prefix p (prefix_from_aug (insert_aug k v aut))
-  ).
-Proof.
-  induction aut as [k' v' | p l IHl r IHr].
-  - intros p H1 H2 H3 H4. split.
-    + simpl. destruct (critical_bit_zer k' k) eqn:E.
-      * simpl. unfold insert_as_branch_aug. assert (take_zer n k' = take_zer n k).
-        { apply critical_bit_zer_take_eq. exact E. } apply critical_bit_zer_ith_neq in E.
-        destruct (ith_zer n k) eqn:E2.
-       -- apply acv_branch.
-         ++ exact H2.
-         ++ simpl. apply prefix_iff_take_eq. rewrite app_length. rewrite PeanoNat.Nat.add_comm.
-            simpl (_ + _). rewrite take_length. apply not_true_is_false in E.
-            rewrite <- H. rewrite <- E. symmetry. apply take_with_ith.
-         ++ apply acv_leaf. exact H1.
-         ++ simpl. apply prefix_iff_take_eq. rewrite app_length. rewrite PeanoNat.Nat.add_comm.
-            simpl (_ + _). rewrite take_length. symmetry. rewrite <- E2. apply take_with_ith.
-       -- apply acv_branch.
-         ++ apply acv_leaf. exact H1.
-         ++ simpl. apply prefix_iff_take_eq. rewrite app_length. rewrite PeanoNat.Nat.add_comm.
-            simpl (_ + _). rewrite take_length. symmetry. rewrite <- E2. apply take_with_ith.
-         ++ exact H2.
-         ++ simpl. apply prefix_iff_take_eq. rewrite app_length. rewrite PeanoNat.Nat.add_comm.
-            simpl (_ + _). rewrite take_length. apply not_false_is_true in E.
-            rewrite <- H. rewrite <- E. symmetry. apply take_with_ith.
-      * apply acv_leaf. inversion H2. exact H0.
-    + split.
-      * simpl. destruct (critical_bit_zer k' k) eqn:E.
-       -- unfold insert_as_branch_aug. unfold insert. unfold insert_as_branch.
-          destruct (ith_zer n k) eqn:E2.
-         ++ simpl. rewrite take_length. reflexivity.
-         ++ simpl. rewrite take_length. reflexivity.
-       -- simpl. inversion H2. apply critical_bit_zer_none_eq in E. rewrite E. reflexivity.
-          exact H0. exact H1.
-      * simpl. destruct (critical_bit_zer k' k) eqn:E.
-       -- unfold insert_as_branch_aug. simpl. simpl in H4.
-          assert (length p <= n).
-          { apply critical_bit_zer_ith_neq in E. apply prefix_iff_take_eq in H3.
-          apply prefix_iff_take_eq in H4. assert (S n <= length p \/ length p <= n).
-          { assert ({n <= length p} + {length p <= n}). apply le_dec. destruct H.
-          apply le_le_S_eq in l. destruct l. left. exact H. right. rewrite H. apply le_n.
-          right. exact l. } destruct H.
-          assert (ith_zer n k = ith_zer n p).
-          { rewrite <- (ith_from_take n (length p)). rewrite H3. reflexivity. exact H. }
-          assert (ith_zer n k' = ith_zer n p).
-          { rewrite <- (ith_from_take n (length p)). rewrite H4. reflexivity. exact H. }
-          rewrite <- H5 in H0. symmetry in H0. apply E in H0. destruct H0. exact H. }
-          assert (is_prefix_fin p (take_zer n k)). { apply is_prefix_zer_fin. split.
-          apply prefix_iff_take_eq. rewrite take_take. apply prefix_iff_take_eq.
-          exact H3. exact H. rewrite take_length. exact H. } destruct (ith_zer n k).
-         ++ simpl. exact H0.
-         ++ simpl. exact H0.
-       -- simpl. simpl in H4. exact H4.
-  - intros p' H1 H2 H3 H4. split.
-    + simpl. destruct (critical_bit_fin k p) eqn:E.
-      * unfold insert_as_branch_aug. destruct (ith_zer n k) eqn:E2.
-       -- apply acv_branch.
-         ++ exact H2.
-         ++ simpl in H4. simpl. replace false with (negb (ith_zer n k)).
-            apply critical_bit_fin_prefix. exact E. rewrite E2. reflexivity.
-         ++ apply acv_leaf. exact H1.
-         ++ simpl. rewrite <- E2. rewrite take_with_ith. apply take_is_prefix.
-       -- apply acv_branch.
-         ++ apply acv_leaf. exact H1.
-         ++ simpl. rewrite <- E2. rewrite take_with_ith. apply take_is_prefix.
-         ++ apply H2.
-         ++ simpl. replace true with (negb (ith_zer n k)).
-            apply critical_bit_fin_prefix. exact E. rewrite E2. reflexivity.
-      * destruct (ith_zer (length p) k) eqn:E2.
-       -- clear IHl. inversion H2. clear H0 H5 H6 p0 l0 r0.
-          assert (is_prefix_zer (p ++ [true]) k). { rewrite <- E2.
-          apply is_prefix_zer_with_ith. apply critical_bit_fin_none_prefix.
-          exact E. }
-          specialize (IHr (p ++ [true]) H1 H9 H H10). destruct IHr as [IH1 [IH2 IH3]].
-          apply acv_branch.
-         ++ exact H7.
-         ++ exact H8.
-         ++ exact IH1.
-         ++ exact IH3.
-       -- clear IHr. inversion H2. clear H0 H5 H6 p0 l0 r0.
-          assert (is_prefix_zer (p ++ [false]) k). { rewrite <- E2.
-          apply is_prefix_zer_with_ith. apply critical_bit_fin_none_prefix.
-          exact E. }
-          specialize (IHl (p ++ [false]) H1 H7 H H8). destruct IHl as [IH1 [IH2 IH3]].
-          apply acv_branch.
-         ++ exact IH1.
-         ++ exact IH3.
-         ++ exact H9.
-         ++ exact H10.
-    + split.
-      * simpl (strip_augCBT (AugBranch _ _ _)). simpl (insert_aug _ _ _).
-        destruct (critical_bit_fin k p) eqn:E.
-       -- unfold insert_as_branch_aug. assert (is_prefix_zerb p k = false).
-          { destruct (is_prefix_zerb p k) eqn:Ep. rewrite is_prefix_zer_iff in Ep.
-          rewrite <- critical_bit_fin_none_prefix in Ep.
-          rewrite E in Ep. discriminate. reflexivity. }
-          assert (is_beforeb (critical_bit_zer p k) (length p) = true). {
-            destruct (is_beforeb (critical_bit_zer p k) (length p)) eqn:E2.
-            reflexivity. unfold is_beforeb in E2. destruct (critical_bit_zer p k) eqn:E3.
-            - apply critical_bit_zer_take_eq in E3. apply Nat.ltb_ge in E2.
-              assert (take_zer (length p) p = take_zer (length p) k).
-              { rewrite <- (take_take (length p) n0 p).
-              rewrite <- (take_take (length p) n0 k). rewrite E3. reflexivity.
-              exact E2. exact E2. } symmetry in H0. rewrite take_full in H0.
-              rewrite <- prefix_iff_take_eq in H0. apply is_prefix_zer_iff in H0.
-              rewrite H0 in H. discriminate.
-            - apply critical_bit_zer_none_prefix in E3. apply is_prefix_zer_iff in E3.
-              rewrite E3 in H. discriminate. }
-            destruct (ith_zer n k) eqn:E4.
-         ++ simpl (strip_augCBT (AugBranch _ _ _)). rewrite take_length. simpl.
-            rewrite H. destruct (is_beforeb (critical_bit_zer p k) (length p)) eqn:E2.
-           ** unfold is_beforeb in E2. destruct (critical_bit_zer p k) eqn:E3.
-            --- unfold insert_as_branch. rewrite critical_bit_zer_comm in E3.
-                apply critical_bit_fin_zer in E. rewrite E3 in E. injection E as E.
-                rewrite E in *. clear E n0. rewrite E4. reflexivity.
-            --- discriminate.
-           ** discriminate.
-         ++ simpl (strip_augCBT (AugBranch _ _ _)). rewrite take_length. simpl.
-            rewrite H. destruct (is_beforeb (critical_bit_zer p k) (length p)) eqn:E2.
-           ** unfold is_beforeb in E2. destruct (critical_bit_zer p k) eqn:E3.
-            --- unfold insert_as_branch. rewrite critical_bit_zer_comm in E3.
-                apply critical_bit_fin_zer in E. rewrite E3 in E. injection E as E.
-                rewrite E in *. clear E n0. rewrite E4. reflexivity.
-            --- discriminate.
-           ** discriminate.
-       -- simpl. assert (is_prefix_zerb p k = true). {
-          apply critical_bit_fin_none_prefix in E. apply is_prefix_zer_iff. exact E. }
-          rewrite H.
-          assert (is_beforeb (critical_bit_augCBT k (AugBranch p l r)) (length p) = false).
-          { apply critical_bit_augCBT_increasing. exact H2. apply is_prefix_zer_iff.
-          exact H. } simpl in H0. rewrite H in H0. rewrite H0.
-          inversion H2. assert (is_prefix_zer (p ++ [ith_zer (length p) k]) k).
-          { apply is_prefix_zer_with_ith. apply critical_bit_fin_none_prefix in E.
-          apply is_prefix_zer_iff. exact H. }
-          destruct (ith_zer (length p) k) eqn:E4.
-         ++ simpl. f_equal. clear IHl. inversion H2.
-            specialize (IHr (p ++ [true]) H1 H10 H12 H11). destruct IHr as [IH1 [IH2 IH3]].
-            exact IH2.
-         ++ simpl. f_equal. clear IHr. inversion H2.
-            specialize (IHl (p ++ [false]) H1 H16 H12 H9). destruct IHl as [IH1 [IH2 IH3]].
-            exact IH2.
-      * simpl in H4. simpl. unfold insert_as_branch_aug. destruct (critical_bit_fin k p) eqn:E.
-       -- assert (n <= length p). { apply length_critical_bit_fin in E.
-          apply le_S in E. apply le_S_n in E. exact E. } apply critical_bit_fin_zer in E.
-          assert (length p' <= n). {
-            assert (ith_zer n k <> ith_zer n p). apply critical_bit_zer_ith_neq in E. exact E.
-            assert ({length p' <= n} + {n <= length p'}). apply le_dec. destruct H5.
-            exact l0. apply le_decide in l0. unfold lt_or_eq in l0. destruct l0. unfold ">" in g.
-            unfold "<" in g. rewrite <- (ith_from_take n (length p')) in H0.
-            rewrite <- (ith_from_take n (length p') p) in H0. apply prefix_iff_take_eq in H3.
-            apply is_prefix_fin_zer in H4. apply prefix_iff_take_eq in H4. rewrite H3 in H0.
-            rewrite H4 in H0. exfalso. apply H0. reflexivity. exact g. exact g. rewrite e.
-            apply le_n. } destruct (ith_zer n k) eqn:E2.
-         ++ simpl. apply is_prefix_zer_fin. split.
-           ** apply prefix_iff_take_eq. rewrite take_take. apply prefix_iff_take_eq. exact H3.
-              exact H0.
-           ** rewrite take_length. exact H0.
-         ++ simpl. apply is_prefix_zer_fin. split.
-           ** apply prefix_iff_take_eq. rewrite take_take. apply prefix_iff_take_eq. exact H3.
-              exact H0.
-           ** rewrite take_length. exact H0.
-       -- assert (prefix_from_aug (if ith_zer (length p) k
-            then AugBranch p l (insert_aug k v r) else AugBranch p (insert_aug k v l) r) = Finite p).
-          { destruct (ith_zer (length p) k). reflexivity. reflexivity. } rewrite H. exact H4.
+  intros p m t k v p' H. generalize dependent p'. induction H.
+  - intros p' H1 H2 H3. unfold insert. unfold critical_bit_CBT. simpl.
+    destruct (critical_bit_zer k k0) eqn:E.
+    + exists (Finite (take_zer n k)). simpl in *. split.
+      * assert (length p' <= n). pose proof (Nat.le_gt_cases (length p') n).
+        destruct H0. assumption. unfold "<" in H0. apply critical_bit_zer_ith_neq in E.
+        apply (ith_from_prefix _ _ n) in H1. apply (ith_from_prefix _ _ n) in H2.
+        rewrite <- H2 in E. apply E in H1. destruct H1. assumption. assumption.
+        apply is_prefix_zer_fin. split. apply prefix_iff_take_eq.
+        apply prefix_iff_take_eq in H2. rewrite take_take. assumption. assumption.
+        rewrite take_length. assumption.
+      * unfold insert_as_branch. pose proof (critical_bit_zer_ith_neq _ _ _ E).
+        pose proof E as Hcb.
+        apply critical_bit_zer_prefix in E.
+        assert (pmCBT_valid (ZeroExt k0) (singleton k0 v0) (Leaf k0 v0)).
+        { constructor. assumption. }
+        assert (pmCBT_valid (ZeroExt k) (singleton k v) (Leaf k v)).
+        { apply pcv_leaf. assumption. }
+        assert (is_prefix (take_zer n k ++ [negb (ith_zer n k)]) (ZeroExt k0)).
+        { simpl. assumption. }
+        assert (is_prefix (take_zer n k ++ [ith_zer n k]) (ZeroExt k)).
+        { simpl. pose proof (is_prefix_zer_with_ith (take_zer n k) k).
+          pose proof (take_is_prefix k n). apply H7 in H8. rewrite take_length in H8.
+          assumption. }
+        rewrite cmap_insert_cbit_singleton with (n := n).
+        -- destruct (ith_zer n k); rewrite <- (take_length n k) at 2;
+           rewrite <- (take_length n k) at 3; econstructor; eassumption.
+        -- assumption.
+    + exists (ZeroExt k). apply (critical_bit_zer_none_eq k k0) in E. subst k0. split.
+      * assumption.
+      * rewrite cmap_insert_eqk_singleton. constructor. assumption.
+      * assumption.
+      * assumption.
+  - intros p' H1 H2 H3. unfold insert. simpl. 
+    destruct ((is_beforeb (critical_bit_CBT k (Branch (length p) l r))) (length p)) eqn:E.
+    + pose proof (low_critbit_on_prefix X k p (Branch (length p) l r)).
+      Print pcv_branch.
+      specialize (H4 (pmCBT_valid_forget_m _ _ _ _ (pcv_branch p pl pr ml mr l r H H0 Hpl Hpr)) E). rewrite H4 in *. apply is_beforeb_true_exists in E. destruct E as [n [H5 H6]].
+      rewrite H5. exists (Finite (take_zer n p)). split.
+      * simpl. simpl in H1. assert (length p' <= n).
+        destruct (le_le_S_dec (length p') n).
+        assumption. apply critical_bit_fin_zer in H5.
+        apply critical_bit_zer_ith_neq in H5. apply prefix_iff_take_eq in H2.
+        apply is_prefix_fin_zer in H1. apply prefix_iff_take_eq in H1.
+        assert (ith_zer n p' = ith_zer n p'). reflexivity. rewrite <- H1 in H7 at 2.
+        rewrite <- H2 in H7 at 1. rewrite ith_from_take in H7.
+        rewrite ith_from_take in H7. apply H5 in H7. destruct H7. assumption.
+        assumption. apply is_prefix_zer_fin. split. apply prefix_iff_take_eq.
+        apply is_prefix_fin_zer in H1. apply prefix_iff_take_eq in H1.
+        rewrite take_take. assumption. assumption. rewrite take_length. assumption.
+      * unfold insert_as_branch.
+        assert (take_zer n k = take_zer n p).
+        { apply critical_bit_fin_zer in H5. apply (critical_bit_zer_take_eq _ _ _ H5). }
+        assert (is_prefix (take_zer n p ++ [negb (ith_zer n k)]) (Finite p)).
+        { simpl. pose proof (critical_bit_fin_prefix _ _ _ H5).          
+          rewrite H7 in H8. assumption. }
+        assert (is_prefix (take_zer n p ++ [ith_zer n k]) (ZeroExt k)).
+        { simpl. rewrite <- H7. rewrite take_with_ith. apply take_is_prefix. }
+        Print pcv_branch.
+        assert (pmCBT_valid (Finite p) (cbit_union (length p) ml mr)
+                  (Branch (length p) l r)).
+        { eapply pcv_branch; eassumption. }
+        destruct (ith_zer n k) eqn:E; erewrite cmap_insert_low_cb_branch;
+          try erewrite E; try eapply pmcv_finite_len_num; try apply take_length;
+          try rewrite H4; try eassumption; try reflexivity; constructor; assumption.
+    + exists (Finite p). split; try assumption. unfold critical_bit_CBT.
+      erewrite cmap_insert_high_cb_branch; try eapply pcv_branch; try eassumption.
+      simpl. apply high_critbit_is_prefix in E;
+        try (eapply pmCBT_valid_forget_m; eapply pcv_branch; eassumption).
+      unfold insert in *.
+      destruct (ith_zer (length p) k) eqn:E2;
+        [edestruct IHpmCBT_valid2 as [pi ?] | edestruct IHpmCBT_valid1 as [pi ?]];
+        try eassumption; try rewrite <- E2; try apply is_prefix_zer_with_ith;
+        try assumption; destruct H4;
+        [eapply pcv_branch with (pr := pi) | eapply pcv_branch with (pl := pi)];
+        try eassumption.
 Qed.
 
-Lemma lookup_some_has_prefix : forall (X : Type) (k : list bool) (v : X) (p : list bool) (l r : augCBT),
-  (OneTerminated k) -> 
-  (augCBT_valid (AugBranch p l r)) ->
-  (lookup k (strip_augCBT (AugBranch p l r)) = Some v) ->
-  (is_prefix_zer p k).
+Theorem lookup_correct : forall (X : Type) (p : prefix) (m : content_map X) (t : CBT)
+                                (k : list bool),
+    OneTerminated k -> pmCBT_valid p m t -> lookup k t = m k.
 Proof.
-  intros X k v p l r. remember (AugBranch p l r) as aut. intros H E. revert Heqaut. generalize p l r.
-  clear p l r. induction E.
-  - intros p0 l0 r0 Heq. discriminate.
-  - simpl. intros p0 l0 r0 Heq. injection Heq as Heq. rewrite <- Heq. clear p0 l0 r0 H0 H1 Heq.
-    assert (L: forall (aut : augCBT),
-      (forall (p : list bool) (l r0 : augCBT),
-       aut = AugBranch p l r0 -> lookup k (strip_augCBT aut) = Some v -> is_prefix_zer p k) ->
-       (is_prefix p (prefix_from_aug aut)) ->
-       (augCBT_valid aut) ->
-       lookup k (strip_augCBT aut) = Some v -> is_prefix_zer p k). {
-      clear IHE1 IHE2 H4 E2 H2 E1 l r H. intros aut IH H1 H2 H3. inversion H2.
-        - rewrite <- H0 in H3. simpl in H3. assert (key_eqb k k0 = true). destruct (key_eqb k k0).
-          reflexivity. discriminate. rewrite <- H0 in H1. simpl in H1. apply key_eqb_iff in H4.
-          rewrite H4. exact H1.
-        - symmetry in H. rewrite H in H1. simpl in H1. pose proof (IH _ _ _ H H3).
-          apply (prefix_zer_trans p p0 k). exact H1. exact H7. 
-    }
-    destruct (ith_zer (length p) k).
-    + apply app_is_prefix in H4. exact (L r IHE2 H4 E2).
-    + apply app_is_prefix in H2. exact (L l IHE1 H2 E1).
-Qed.
-
-Lemma insert_content_aug : forall (X : Type) (k : list bool) (v : X) (aut : augCBT),
-  (OneTerminated k) -> (augCBT_valid aut) ->
-  (equal_content (content_aug (insert_aug k v aut)) (insert_map k v (content_aug aut))).
-Proof.
-  intros X k v. induction aut.
-  - intros H1 H2. unfold equal_content. intro k'. unfold insert_map. unfold content_aug. simpl.
-    destruct (critical_bit_zer k0 k) eqn:E.
-    + unfold insert_as_branch_aug. destruct (ith_zer n k) eqn:E2.
-      * simpl. rewrite take_length. destruct (key_eqb k' k) eqn:E3.
-       -- apply key_eqb_iff in E3. rewrite E3 in *. rewrite E2. reflexivity.
-       -- destruct (ith_zer n k') eqn:E4. assert (k' <> k0). intro. rewrite <- H in E.
-          apply critical_bit_zer_ith_neq in E. apply E. rewrite E2. rewrite E4. reflexivity.
-          apply key_eqb_niff in H. rewrite H. reflexivity. reflexivity.
-      * simpl. rewrite take_length. destruct (key_eqb k' k) eqn:E3.
-       -- apply key_eqb_iff in E3. rewrite E3. rewrite E2. reflexivity.
-       -- destruct (ith_zer n k') eqn:E4. reflexivity. assert (k' <> k0). intro.
-          rewrite <- H in E. apply critical_bit_zer_ith_neq in E. apply E.
-          rewrite E2. rewrite E4. reflexivity. apply key_eqb_niff in H. rewrite H. reflexivity.
-    + inversion H2. apply (critical_bit_zer_none_eq _ _ H0 H1) in E. rewrite E in *.
-      simpl. destruct (key_eqb k' k). reflexivity. reflexivity.
-  - intros H1 H2. simpl. destruct (critical_bit_fin k p) eqn:E.
-    (* inserting k creates a new top-level branch *)
-    + clear IHaut1 IHaut2. unfold insert_as_branch_aug. unfold equal_content. intros k' H.
-      unfold insert_map. unfold content_aug. simpl. destruct (key_eqb k' k) eqn:E2.
-      * apply key_eqb_iff in E2. rewrite E2 in *. destruct (ith_zer n k) eqn:E3.
-       -- simpl. rewrite take_length. rewrite E3. rewrite key_eqb_reflx. reflexivity.
-       -- simpl. rewrite take_length. rewrite E3. rewrite key_eqb_reflx. reflexivity.
-      * remember (AugBranch p aut1 aut2) as aut. destruct (lookup k' (strip_augCBT aut)) eqn:E3.
-       -- assert (is_prefix_zer p k'). rewrite Heqaut in H2. rewrite Heqaut in E3.
-          exact (lookup_some_has_prefix _ _ x _ _ _ H H2 E3). assert (ith_zer n k <> ith_zer n k').
-          { intro. apply prefix_iff_take_eq in H0. assert (S n <= length p).
-          apply (length_critical_bit_fin _ _ _ E). apply critical_bit_fin_zer in E.
-          apply critical_bit_zer_ith_neq in E. apply (ith_from_take _ _ k') in H4. rewrite H0 in H4.
-          apply E. rewrite H3. rewrite H4. reflexivity. } rewrite Heqaut in E3. pose proof E3. simpl in E3.
-          rewrite E3. clear E3 H0. destruct (ith_zer n k).
-         ++ simpl. rewrite take_length. apply not_eq_sym in H3. apply not_true_is_false in H3. rewrite H3.
-          rewrite Heqaut. exact H4.
-         ++ simpl. rewrite take_length. apply not_eq_sym in H3. apply not_false_is_true in H3. rewrite H3.
-          rewrite Heqaut. exact H4.
-       -- pose proof E3. rewrite Heqaut in E3. simpl in E3. rewrite E3. clear E3. destruct (ith_zer n k).
-         ++ simpl. rewrite take_length. rewrite H0. rewrite E2. destruct (ith_zer n k').
-            reflexivity. reflexivity.
-         ++ simpl. rewrite take_length. rewrite H0. rewrite E2. destruct (ith_zer n k').
-            reflexivity. reflexivity.
-    (* k is inserted below the current top-level branch *)
-    + unfold equal_content. intros k' H. unfold insert_map. unfold content_aug.
-      inversion H2. specialize (IHaut1 H1 H5 k' H) as IH1. specialize (IHaut2 H1 H7 k' H) as IH2.
-      clear IHaut1 IHaut2 H3 l H4 r p0 H0.
-      unfold content_aug in *. unfold insert_map in *. destruct (ith_zer (length p) k) eqn:E2.
-      * simpl. destruct (ith_zer (length p) k') eqn:E3.
-       -- exact IH2.
-       -- destruct (key_eqb k' k) eqn:E4. apply key_eqb_iff in E4. rewrite E4 in E3. rewrite E3 in E2.
-          discriminate. reflexivity.
-      * simpl. destruct (ith_zer (length p) k') eqn:E3.
-       -- destruct (key_eqb k' k) eqn:E4. apply key_eqb_iff in E4. rewrite E4 in E3. rewrite E3 in E2.
-          discriminate. reflexivity.
-       -- exact IH1.
-Qed.
-
-Lemma insert_aug_match_com : forall (X : Type) (k : list bool) (v : X) (aut : augCBT),
-  (OneTerminated k) -> (augCBT_valid aut) ->
-  (strip_augCBT (insert_aug k v aut) = insert k v (strip_augCBT aut)).
-Proof.
-  intros X k v aut H1 H2. unfold insert. pose proof (insert_aug_match X k v aut [] H1 H2).
-  specialize (H (ipfz1 _) (is_prefix_nil _)). destruct H as [_ [H _]].
-  rewrite (critical_bit_aug_match _ _ _ H2) in H. exact H.
-Qed.
-
-Lemma insert_aug_valid : forall (X : Type) (k : list bool) (v : X) (aut : augCBT),
-  (OneTerminated k) -> (augCBT_valid aut) -> (augCBT_valid (insert_aug k v aut)).
-Proof.
-  intros X k v aut H1 H2. unfold insert. pose proof (insert_aug_match X k v aut [] H1 H2).
-  specialize (H (ipfz1 _) (is_prefix_nil _)). destruct H as [H _]. exact H.
+  intros. induction H0.
+  - unfold singleton. rewrite key_eqb_sym. reflexivity.
+  - unfold cbit_union. simpl. destruct (ith_zer (length p) k); assumption.
 Qed.
